WIP

backend/RTLC.v
@@ -88,14 +88,14 @@ Section MODSEM.
 
   Variable skenv_link: SkEnv.t.
   Variable p: program.
-  Let skenv: SkEnv.t := skenv_link.(SkEnv.project) p.(internals).
+  Let skenv: SkEnv.t := skenv_link.(SkEnv.project) p.(defs).
   Let ge: genv := skenv.(SkEnv.revive) p.
 
   Inductive at_external: state -> Args.t -> Prop :=
   | at_external_intro
       stack fptr_arg sg_arg vs_arg m0
       (EXTERNAL: ge.(Genv.find_funct) fptr_arg = None)
-      (SIG: skenv_link.(Genv.find_funct) fptr_arg = Some (Internal sg_arg))
+      (SIG: exists skd, skenv_link.(Genv.find_funct) fptr_arg = Some skd /\ SkEnv.sig_compat skd sg_arg)
     :
       at_external (Callstate stack fptr_arg sg_arg vs_arg m0)
                   (Args.mk fptr_arg vs_arg m0)
@@ -213,7 +213,7 @@ Section MODULE.
     |}
   .
   Next Obligation.
-    rewrite Sk.of_program_internals.
+    rewrite Sk.of_program_defs.
     eapply SkEnv.project_impl_spec; eauto.
   Qed.
 
