proof/AdequacyLocal.v
@@ -10,7 +10,7 @@ Require Import Integers.
 Require Import Events.
 
 Require Import Skeleton ModSem Mod Sem.
-Require Import SimDef SimSymb SimMem SimMod SimModSem SimProg (* SimLoad *) SimProg.
+Require Import SimSymb SimMem SimMod SimModSem SimProg (* SimLoad *) SimProg.
 Require Import SemProps Ord.
 
 Set Implicit Arguments.
@@ -20,7 +20,13 @@ Set Implicit Arguments.
 
 
 
-
+(* TODO: move to coqlibc *)
+Ltac revert_until_bar :=
+  on_last_hyp ltac:(fun id' => match (type of id') with
+                               | bar_True => idtac
+                               | _ => revert id'; revert_until_bar
+                               end)
+.
 
 
 
@@ -103,107 +109,6 @@ Section SIMGE.
     - apply in_map_iff. esplits; eauto.
  
   Qed.
- 
-
-
-  Lemma find_fptr_owner_bsim
-        sm0 ge_src ge_tgt
-        (SIMGE: sim_ge sm0 ge_src ge_tgt)
-        fptr_src fptr_tgt
-        (SIMFPTR: SimMem.sim_val sm0 fptr_src fptr_tgt)
-        ms_tgt
-        (FINDTGT: Ge.find_fptr_owner ge_tgt fptr_tgt ms_tgt)
-        (SAFESRC: exists ms_src, Ge.find_fptr_owner ge_src fptr_src ms_src)
-    :
-      exists msp,
-        <<FINDSRC: Ge.find_fptr_owner ge_src fptr_src msp.(ModSemPair.src)>>
-        /\ <<FINDTGT: ModSemPair.tgt msp = ms_tgt>>
-        /\ <<SIMMS: ModSemPair.sim msp>>
-        /\ <<SIMSKENV: ModSemPair.sim_skenv msp sm0>>
-  .
-  Proof.
-    inv SIMGE.
-    { des. inv SAFESRC; ss. }
-    rewrite Forall_forall in *.
-    {
-      assert(SAFESRC0: fptr_src <> Vundef).
-      { ii; ss; clarify. des; ss. inv SAFESRC. ss. }
-      clear SAFESRC.
-
-      inv FINDTGT.
-      rewrite in_map_iff in MODSEM. des. rename x into msp.
-      clarify.
-      
-      specialize (SIMMSS msp). exploit SIMMSS; eauto. clear SIMMSS. intro SIMMS.
-      specialize (SIMSKENV msp). exploit SIMSKENV; eauto. clear SIMSKENV. intro SIMSKENV.
-      exploit SimSymb.sim_skenv_func_bisim; eauto. intro SIMFUNC; des.
-      inv SIMFUNC.
-      exploit FUNCBSIM; try apply PROGRESS; eauto. i; des. clarify. clear_tac. inv SIM.
-      exists msp. esplits; eauto.
-      { econs; eauto. rewrite in_map_iff; eauto. }
-    }
-  Qed.
-
-  Lemma find_fptr_owner_bsim_deprecated
-        sm0 ge_src ge_tgt
-        (SIMGE: sim_ge sm0 ge_src ge_tgt)
-        fptr_src fptr_tgt
-        (SIMFPTR: SimMem.sim_val sm0 fptr_src fptr_tgt)
-        ms_tgt
-        (FINDTGT: Ge.find_fptr_owner ge_tgt fptr_tgt ms_tgt)
-        ms_src
-        (SAFESRC: Ge.find_fptr_owner ge_src fptr_src ms_src)
-    :
-      exists msp,
-        <<SRC: ModSemPair.src msp = ms_src>>
-        /\ <<TGT: ModSemPair.tgt msp = ms_tgt>>
-        /\ <<SIMMS: ModSemPair.sim msp>>
-        /\ <<SIMSKENV: ModSemPair.sim_skenv msp sm0>>
-  .
-  Proof.
-  (*   inv SIMGE. *)
-  (*   rewrite Forall_forall in *. *)
-  (*   clear SAFESRC. *)
-  (*   inv FINDTGT. *)
-  (*   rewrite in_map_iff in MODSEM. des. rename x into msp. *)
-  (*   specialize (SIMMSS msp). exploit SIMMSS; eauto. clear SIMMSS. intro SIMMS. *)
-  (*   specialize (SIMSKENV msp). exploit SIMSKENV; eauto. clear SIMSKENV. intro SIMSKENV. *)
-  (*   clarify. *)
-  (*   esplits; eauto. *)
-
-
-  (*   inv SIMGE. *)
-  (*   rewrite Forall_forall in *. *)
-  (*   dup SAFESRC. *)
-  (*   inv SAFESRC. *)
-  (*   rewrite in_map_iff in MODSEM. des. rename x into msp. *)
-  (*   specialize (SIMMSS msp). exploit SIMMSS; eauto. clear SIMMSS. intro SIMMS. *)
-  (*   specialize (SIMSKENV msp). exploit SIMSKENV; eauto. clear SIMSKENV. intro SIMSKENV. *)
-
-  (*   inv FINDTGT. rewrite in_map_iff in *. des. rename msp into _msp. rename x into msp. clarify. *)
-  (*   exploit SimSymb.sim_skenv_func_bsim; eauto. intro SIMFUNC; des. *)
-  (*   inv SIMFUNC. exploit FUNCBSIM; eauto. i; des. clear_tac. inv SIM. *)
-  (*   ttttttttttt *)
-
-  (*   assert(exists blk_tgt, fptr_tgt = Vptr blk_tgt Ptrofs.zero true). *)
-  (*   { inv FINDTGT. esplits; eauto. } des. clarify. *)
-  (*   exploit SimSymb.sim_skenv_def_fsim; eauto. intro SIMDEF; des. *)
-  (*   inv SIMDEF. exploit DEFFSIM; eauto. i; des. clear_tac. inv SIM. inv SIM0. *)
-
-  (*   assert(FINDSRC: Ge.find_fptr_owner (map ModSemPair.tgt msps) *)
-  (*                                      (Vptr blk_tgt Ptrofs.zero true) msp.(ModSemPair.tgt)). *)
-  (*   { econs; eauto. rewrite in_map_iff. esplits; eauto. } *)
-  (*   esplits; eauto. *)
-  (*   assert(exists tp tsk, tp.(Sem.semantics).(globalenv) = (map ModSemPair.tgt msps) /\ link_sk tp = Some tsk). *)
-  (*   { admit "". } *)
-  (*   des. *)
-  (*   eapply find_fptr_owner_determ with (p:= tp); eauto. *)
-  (*   { ss. des_ifs. rewrite H. eauto. } *)
-  (*   { ss. des_ifs. rewrite H. eauto. } *)
-  (* Qed. *)
-  Abort.
-
-
 
   Lemma msp_in_sim
         sm0 ge_src ge_tgt
@@ -436,8 +341,8 @@ Section ADQMATCH.
   Variable sk_link_src sk_link_tgt: Sk.t.
   Hypothesis LINKSRC: (link_sk p_src) = Some sk_link_src.
   Hypothesis LINKTGT: (link_sk p_tgt) = Some sk_link_tgt.
-  Let sem_src := Sem.semantics p_src.
-  Let sem_tgt := Sem.semantics p_tgt.
+  Let sem_src := Sem.sem p_src.
+  Let sem_tgt := Sem.sem p_tgt.
   Compute sem_src.(Smallstep.state).
 
   Print Frame.t.
@@ -447,19 +352,17 @@ Section ADQMATCH.
   (* (SimMem.t is lifted. lifting/unlifting is caller's duty) *)
   (* Simulation can go continuation when SimMem.t bigger than argument is given, (after unlifting it) *)
   (* with after_external fed with regsets sent. *)
-  Inductive lxsim_stack: regset -> regset -> SimMem.t ->
+  Inductive lxsim_stack: SimMem.t ->
                          list Frame.t -> list Frame.t -> Prop :=
   | lxsim_stack_nil
-      rs_init_src rs_init_tgt sm0
+      sm0
     :
-      lxsim_stack rs_init_src rs_init_tgt sm0 [] []
+      lxsim_stack sm0 [] []
   | lxsim_stack_cons
       tail_src tail_tgt tail_sm
-      rs_init_src rs_init_tgt
-      (STACK: lxsim_stack rs_init_src rs_init_tgt tail_sm tail_src tail_tgt)
+      (STACK: lxsim_stack tail_sm tail_src tail_tgt)
       ms_src lst_src0
       ms_tgt lst_tgt0
-      rs_arg_src rs_arg_tgt
       sm_arg
       (MWF: SimMem.wf sm_arg)
       (GE: sim_ge sm_arg sem_src.(globalenv) sem_tgt.(globalenv))
@@ -467,52 +370,31 @@ Section ADQMATCH.
       sm_init
       (MLE: SimMem.le (SimMem.lift sm_arg) sm_init)
       (K: forall
-          sm_ret rs_ret_src rs_ret_tgt
-          (MEMLE: SimMem.le (SimMem.lift sm_arg) sm_ret)
-          (MEMWF: SimMem.wf sm_ret)
-          (RSREL: sm_ret.(SimMem.sim_regset) rs_ret_src rs_ret_tgt)
-          (SAFESRC: exists lst_src1,
-              <<AFTERSRC: ms_src.(ModSem.after_external) lst_src0 rs_arg_src rs_ret_src
-                                                         (sm_ret.(SimMem.src))
-                                                         lst_src1>>)
+          sm_ret retv_src retv_tgt
+          (MLE: SimMem.le (SimMem.lift sm_arg) sm_ret)
+          (MWF: SimMem.wf sm_ret)
+          (SIMRETV: sim_retv retv_src retv_tgt sm_ret)
+          lst_src1
+          (AFTERSRC: ms_src.(ModSem.after_external) lst_src0 retv_src lst_src1)
         ,
-          (<<KSTEP: forall
-              lst_tgt1
-              (AFTERTGT: ms_tgt.(ModSem.after_external) lst_tgt0 rs_arg_tgt rs_ret_tgt (sm_ret.(SimMem.tgt))
-                                                        lst_tgt1)
-            ,
-              exists i0 lst_src1,
-                (<<AFTERSRC:
-                   ms_src.(ModSem.after_external) lst_src0 rs_arg_src rs_ret_src (sm_ret.(SimMem.src))
-                                                  lst_src1>>)
-                /\
-                (<<LXSIM: lxsim ms_src ms_tgt rs_init_src rs_init_tgt tail_sm
-                                i0 lst_src1 lst_tgt1 (sm_arg.(SimMem.unlift) sm_ret)>>)>>)
-          /\
-          (<<KPROGRESS: (* forall *)
-              (* st_src1 *)
-              (* (AFTERSRC: ms_src.(ModSem.after_external) lst_src0 rs_arg_src rs_ret_src (sm_ret.(SimMem.src)) *)
-              (*                                           st_src1) *)
-            (* , *)
-              exists lst_tgt1,
-                (<<AFTERTGT:
-                   ms_tgt.(ModSem.after_external) lst_tgt0 rs_arg_tgt rs_ret_tgt (sm_ret.(SimMem.tgt))
-                                                  lst_tgt1>>)>>))
+          exists i1 lst_tgt1,
+            (<<AFTERTGT: ms_tgt.(ModSem.after_external) lst_tgt0 retv_tgt lst_tgt1>>)
+            /\
+            (<<LXSIM: lxsim ms_src ms_tgt tail_sm i1 lst_src1 lst_tgt1 (sm_arg.(SimMem.unlift) sm_ret)>>))
     :
-      lxsim_stack rs_arg_src rs_arg_tgt
-                  sm_init
-                  ((Frame.mk ms_src rs_init_src lst_src0) :: tail_src)
-                  ((Frame.mk ms_tgt rs_init_tgt lst_tgt0) :: tail_tgt)
+      lxsim_stack sm_init
+                  ((Frame.mk ms_src lst_src0) :: tail_src)
+                  ((Frame.mk ms_tgt lst_tgt0) :: tail_tgt)
 
   .
 
   Lemma lxsim_stack_le
-        rs_init_src rs_init_tgt sm0 frs_src frs_tgt
-        (SIMSTACK: lxsim_stack rs_init_src rs_init_tgt sm0 frs_src frs_tgt)
+        sm0 frs_src frs_tgt
+        (SIMSTACK: lxsim_stack sm0 frs_src frs_tgt)
         sm1
         (MLE: SimMem.le sm0 sm1)
     :
-      <<SIMSTACK: lxsim_stack rs_init_src rs_init_tgt sm1 frs_src frs_tgt>>
+      <<SIMSTACK: lxsim_stack sm1 frs_src frs_tgt>>
   .
   Proof.
     inv SIMSTACK.
@@ -526,32 +408,31 @@ Section ADQMATCH.
       sm0
       (GE: sim_ge sm0 sem_src.(globalenv) sem_tgt.(globalenv))
       tail_src tail_tgt tail_sm
-      rs_init_src rs_init_tgt
-      (STACK: lxsim_stack rs_init_src rs_init_tgt tail_sm tail_src tail_tgt)
+      (STACK: lxsim_stack tail_sm tail_src tail_tgt)
       (MLE: SimMem.le tail_sm sm0)
       i0
       ms_src lst_src
       ms_tgt lst_tgt
-      (TOP: lxsim ms_src ms_tgt rs_init_src rs_init_tgt tail_sm
+      (TOP: lxsim ms_src ms_tgt tail_sm
                   i0 lst_src lst_tgt sm0)
     :
       lxsim_lift i0
-                 (State ((Frame.mk ms_src rs_init_src lst_src) :: tail_src))
-                 (State ((Frame.mk ms_tgt rs_init_tgt lst_tgt) :: tail_tgt))
+                 (State ((Frame.mk ms_src lst_src) :: tail_src))
+                 (State ((Frame.mk ms_tgt lst_tgt) :: tail_tgt))
                  sm0
   | lxsim_lift_callstate
        sm_arg
        (GE: sim_ge sm_arg sem_src.(globalenv) sem_tgt.(globalenv))
        tail_src tail_tgt tail_sm
-       rs_arg_src rs_arg_tgt
-       (STACK: lxsim_stack rs_arg_src rs_arg_tgt tail_sm tail_src tail_tgt)
+       (STACK: lxsim_stack tail_sm tail_src tail_tgt)
        (MLE: SimMem.le tail_sm sm_arg)
        (MWF: SimMem.wf sm_arg)
-       (SIMRS: (SimMem.sim_regset) sm_arg rs_arg_src rs_arg_tgt)
+       args_src args_tgt
+       (SIMARGS: sim_args args_src args_tgt sm_arg)
     :
       lxsim_lift idx_bot
-                 (Callstate rs_arg_src sm_arg.(SimMem.src) tail_src)
-                 (Callstate rs_arg_tgt sm_arg.(SimMem.tgt) tail_tgt)
+                 (Callstate args_src tail_src)
+                 (Callstate args_tgt tail_tgt)
                  sm_arg
   .
 
@@ -581,8 +462,8 @@ Section ADQINIT.
   Let p_tgt := pp.(ProgPair.tgt).
   Let lxsim_lift := (@lxsim_lift _ _ p_src p_tgt).
   Hint Unfold lxsim_lift.
-  Let sem_src := Sem.semantics p_src.
-  Let sem_tgt := Sem.semantics p_tgt.
+  Let sem_src := Sem.sem p_src.
+  Let sem_tgt := Sem.sem p_tgt.
   Print Sem.initial_state.
 
   Theorem init_lxsim_lift_forward
@@ -594,6 +475,7 @@ Section ADQINIT.
         /\ <<SIM: lxsim_lift idx st_init_src st_init_tgt sm_init>>
   .
   Proof.
+    ss.
     inv INITSRC; ss.
     rename sk_link into sk_link_src.
     rename INITSK into INITSKSRC. rename INITMEM into INITMEMSRC.
@@ -602,27 +484,21 @@ Section ADQINIT.
     exploit init_sim_ge_strong; eauto. i; des. clarify.
     ss. des_ifs.
 
-    assert(SIMFPTR: SimMem.sim_val sm_init (Genv.symbol_address (Genv.globalenv sk_link_src)
-                                                                (prog_main sk_link_src) Ptrofs.zero)
-                                   (Genv.symbol_address (Genv.globalenv sk_link_tgt)
-                                                        (prog_main sk_link_tgt) Ptrofs.zero)).
-    { admit "strengthen sim_skenv specs". }
-
-    assert(SIMRS: SimMem.sim_regset sm_init
-        (init_regs (Genv.symbol_address (Sk.load_skenv sk_link_src) (prog_main sk_link_src) Ptrofs.zero))
-        (init_regs (Genv.symbol_address (Sk.load_skenv sk_link_tgt) (prog_main sk_link_tgt) Ptrofs.zero))).
-    { u. ii. ss.
-      unfold Pregmap.set.
-      des_ifs.
-      - admit "strengthen sim_val".
-      - admit "strengthen sim_val".
-      - admit "strengthen sim_val".
-    }
+    set(Args.mk (Genv.symbol_address (Sk.load_skenv sk_link_src) (prog_main sk_link_src) Ptrofs.zero)
+                [] sm_init.(SimMem.src)) as args_src in *.
+    set(Args.mk (Genv.symbol_address (Sk.load_skenv sk_link_tgt) (prog_main sk_link_tgt) Ptrofs.zero)
+                [] sm_init.(SimMem.tgt)) as args_tgt in *.
+    assert(SIMARGS: sim_args args_src args_tgt sm_init).
+    { econs; ss; eauto. admit "strengthen sim_skenv specs". }
 
     esplits; eauto.
     - econs; ss; cycle 1.
       { ii. eapply initial_state_determ; ss; eauto. }
       econs; eauto.
+      apply_all_once SimSymb.sim_skenv_func_bisim. des. inv SIMSKENV.
+      exploit FUNCFSIM; eauto.
+      { apply SIMARGS. }
+      i; des. clarify.
     - econs; eauto.
       + ss. des_ifs.
       + econs; eauto.
@@ -671,8 +547,8 @@ Section ADQSTEP.
   Let p_tgt := pp.(ProgPair.tgt).
   Let lxsim_lift := (@lxsim_lift _ _ p_src p_tgt).
   Hint Unfold lxsim_lift.
-  Let sem_src := Sem.semantics p_src.
-  Let sem_tgt := Sem.semantics p_tgt.
+  Let sem_src := Sem.sem p_src.
+  Let sem_tgt := Sem.sem p_tgt.
   Variable sk_link_src sk_link_tgt: Sk.t.
   Hypothesis LINKSRC: (link_sk p_src) = Some sk_link_src.
   Hypothesis LINKTGT: (link_sk p_tgt) = Some sk_link_tgt.
@@ -692,45 +568,62 @@ Section ADQSTEP.
     pcofix CIH. i. pfold.
     inv LXSIM; ss; cycle 1.
     { (* init *)
-      des_ifs. left.
+      des_ifs. right.
+      econs; eauto; cycle 2.
+      { ii.
+        specialize (SAFESRC _ (star_refl _ _ _)). des; ss.
+        - inv SAFESRC.
+        - des_ifs. right. inv SAFESRC.
+          exploit find_fptr_owner_fsim; eauto. { apply SIMARGS. } i; des. clarify.
+          inv SIMMS.
+          inv MSFIND. inv FINDTGT.
+          exploit SIM; eauto. i; des.
+          exploit INITPROGRESS; eauto. i; des.
+          esplits; eauto.
+          econs; eauto.
+          econs; eauto.
+      }
+      { i. ss. inv FINALTGT. }
+      i.
       econs; eauto.
-      { ii. ss. inv FINALSRC. }
-      econs; eauto; cycle 1.
-      { eapply callstate_receptive_at. }
-      ii. ss. des_ifs.
-      inv STEPSRC.
-      exploit find_fptr_owner_fsim; eauto. i; des. clarify.
-      inv MSFIND. inv FINDTGT.
+      i. inv STEPTGT.
+      specialize (SAFESRC _ (star_refl _ _ _)). des.
+      { inv SAFESRC. }
+      bar.
+      inv SAFESRC.
+      ss. des_ifs.
+      bar.
+      exploit find_fptr_owner_fsim; eauto. { apply SIMARGS. } i; des. clarify.
+      exploit find_fptr_owner_determ; ss; eauto.
+      { rewrite Heq. apply FINDTGT. }
+      { rewrite Heq. apply MSFIND. }
+      i; des. clarify.
+
+      clears st_init0; clear st_init0.
+      (* revert_until_bar. *)
+      (* on_last_hyp ltac:(fun H => clear H). *)
+      (* clear_until_bar. *)
+      (* on_last_hyp ltac:(fun H => clear H). *)
+      (* i. *)
+
       inv SIMMS.
-
-
       specialize (SIM sm0).
+      inv MSFIND. inv MSFIND0.
       exploit SIM; eauto. i; des.
 
-      (* specialize (SIM (SimMem.lift sm0)). *)
-      (* exploit SIM; eauto. *)
-      (* { eapply SimMem.lift_sim_val; eauto. } *)
-      (* { ii. eapply SimMem.lift_sim_val; eauto. } *)
-      (* { eapply SimMem.lift_wf; eauto. } *)
-      (* { u. eapply SimSymb.mlift_preserves_sim_skenv; eauto. } *)
-      (* { ss. erewrite SimMem.lift_src. eauto. } *)
-      (* i; des. *)
-
+      exploit INITBSIM; eauto. i; des.
 
       esplits; eauto.
-      - left. eapply plus_one.
-        econs; eauto; cycle 1.
-        + econs; eauto.
-          * ss. des_ifs. econs; eauto; ss.
-          (* * erewrite SimMem.lift_tgt in INITTGT. eauto. *)
-        + eapply callstate_determinate_at; eauto.
-      - instantiate (1:= idx_init).
-        right. eapply CIH.
+      - left. apply plus_one. econs; eauto. econs; eauto.
+      - right. eapply CIH.
         instantiate (1:= sm_init).
-        econs 1; try apply SIM0; eauto.
+        econs; try apply SIM0. eauto.
         + ss. des_ifs. eapply mle_preserves_sim_ge; eauto.
         + eapply lxsim_stack_le; eauto.
+        + ss.
+
     }
+
     rewrite LINKSRC in *. rewrite LINKTGT in *.
     punfold TOP. inv TOP.
 
@@ -748,7 +641,7 @@ Section ADQSTEP.
           { exfalso. eauto. }
           { exfalso. eapply SAFESRC0. u. eauto. }
           exploit STEP; eauto. i; des_safe.
-          exists i1, (State ((Frame.mk ms_tgt rs_init_tgt st_tgt1) :: tail_tgt)).
+          exists i1, (State ((Frame.mk ms_tgt st_tgt1) :: tail_tgt)).
           esplits; eauto.
           { des.
             - left. eapply lift_dplus; eauto.
@@ -771,7 +664,7 @@ Section ADQSTEP.
         * econs 1; eauto.
           ii. inv STEPTGT; ModSem.tac.
           ss. exploit STEP; eauto. i; des_safe.
-          exists i1, (State ((Frame.mk ms_src rs_init_src st_src1) :: tail_src)).
+          exists i1, (State ((Frame.mk ms_src st_src1) :: tail_src)).
           esplits; eauto.
           { des.
             - left. eapply lift_plus; eauto.
@@ -787,123 +680,73 @@ Section ADQSTEP.
 
 
     - (* call *)
-      right.
-      econs; eauto; swap 2 3.
-      { (* final *)
-        ii. inv FINALTGT. ss. exfalso. eapply ModSem.call_return_disjoint; eauto. esplits; eauto. }
-      { (* progress *)
-        ii. right. u in SAFESRC. des.
-        exploit CALLBSIM; eauto. i; des.
-        specialize (SAFESRC0 _ (star_refl _ _ _)). des.
-        { inv SAFESRC0. ss. exfalso. eapply ModSem.call_return_disjoint; eauto. u. esplits; eauto. }
-        ss; des_ifs.
-        inv SAFESRC0; ss; ModSem.tac.
-        esplits; eauto. econs; ss; eauto. }
-
-      (* ii. unfold safe in *. ss. specialize (SAFESRC _ (star_refl _ _ _)). des. *)
-      (* { admit "final forward". } *)
-      (* des_ifs. *)
-
-      (* inv SAFESRC; ss; cycle 1. *)
-      (* { exfalso. eapply ModSem.at_external_final_machine_disjoint; try apply FINAL; eauto. } *)
-      (* { exfalso. eapply ModSem.step_at_external_disjoint; try apply FINAL; eauto. } *)
-
-      econs 1; ss; eauto. i. des_ifs.
-      inv STEPTGT; ss; ModSem.tac.
-      clear SAFESRC.
-      rename rs_arg into rs_arg_tgt.
-      exploit CALLBSIM; eauto. i; des.
-
+      left.
+      econs; eauto.
+      { ii. inv FINALSRC. ss. ModSem.tac. }
+      econs; eauto; cycle 1.
+      { eapply lift_receptive_at. admit "Add in ModSem.v". }
+      i.
+      inv STEPSRC; ss; ModSem.tac.
+      exploit CALLFSIM; eauto.
+      i; des.
       eapply mle_preserves_sim_ge with (sm2:= sm_arg) in GE; eauto.
-      (* Note: Coq bug STILL not fixed!!! there is no name like sm2. *)
-
-      clarify.
       esplits; eauto.
-      + left. apply plus_one. econs; ss; eauto.
+      + left. apply plus_one.
+        econs; ss; eauto.
+        { admit "eapply lift_determinate_at // Add in ModSem.v". }
+        des_ifs.
+        econs 1; eauto.
       + right. eapply CIH; eauto.
         {
           instantiate (1:= (SimMem.lift sm_arg)).
-          erewrite <- SimMem.lift_src. erewrite <- SimMem.lift_tgt.
           econs 2; eauto.
           * ss. des_ifs. eapply mlift_preserves_sim_ge; eauto.
           * instantiate (1:= (SimMem.lift sm_arg)).
             econs; [eassumption|..]; revgoals.
-            { ii. exploit K; eauto. i; des_safe. esplits; eauto.
-              ii. exploit KSTEP; eauto. i; des_safe. pclearbot. esplits; eauto.
-            }
+            { ii. exploit K; eauto. i; des_safe. pclearbot. esplits; eauto. }
             { reflexivity. }
             { etransitivity; eauto. }
             { ss. des_ifs. }
             { eauto. }
           * reflexivity.
           * eapply SimMem.lift_wf; eauto.
-          * ii. eapply SimMem.lift_sim_val; eauto. 
+          * inv SIMARGS. econs; ss; eauto.
+            { eapply SimMem.lift_sim_val; eauto. }
+            { admit "eapply SimMem.lift_sim_val_list; eauto.". }
+            { erewrite SimMem.lift_src. ss. }
+            { erewrite SimMem.lift_tgt. ss. }
         }
 
 
     - (* return *)
-      des_ifs.
-      right.
-      econs; eauto; swap 2 3.
-      { (* final *)
-        ii. inv FINALTGT0. ss. des_ifs.
-        esplits; [apply star_refl|]; eauto.
+      left.
+      econs; eauto.
+      { ii. ss. inv FINALSRC0. ss. determ_tac ModSem.final_frame_dtm. clear_tac.
         inv STACK.
         econs; ss; eauto.
-        - admit "obligate to SimMem.val".
-        - admit "obligate to SimMem.val".
+        - econs; ss; eauto.
+          admit "obligate to SimMem.val".
+        - i. inv FINAL0; inv FINAL1; ss.
+          exploit ModSem.final_frame_dtm; [apply FINAL|apply FINAL0|..]. i; clarify.
+          congruence.
+        - ii. des_ifs.
+          inv H; ss; ModSem.tac.
       }
-      { (* progress *)
-        ii.
-        specialize (SAFESRC _ (star_refl _ _ _)). des.
-        { left. inv SAFESRC. inv STACK. ss.
-          determ_tac ModSem.final_frame_dtm. clear_tac.
-          esplits; eauto. econs; eauto.
-          - admit "obligate to SimMem.val".
-          - admit "obligate to SimMem.val". }
-
-        right. ss. des_ifs.
-        inv SAFESRC; ss.
-        { exfalso. 
-          eapply ModSem.call_return_disjoint; eauto. esplits; eauto. }
-        { exfalso.
-          eapply ModSem.step_return_disjoint; eauto. esplits; eauto. }
-        determ_tac ModSem.final_frame_dtm. clear_tac.
-        bar.
-        move AFTER at bottom.
-        move STACK at bottom.
-        inv STACK. ss.
-        exploit K; try apply RSREL; eauto.
-        { etransitivity; eauto. }
-        { erewrite <- mcompat_src in *; eauto. }
-        i; des.
-        esplits; eauto.
-        econs 4; ss; eauto.
-        erewrite <- mcompat_tgt in *; eauto.
-      }
-      i.
-      econs 1; eauto. ss. des_ifs.
-      ii. inv STEPTGT; ss.
-      { exfalso. eapply ModSem.call_return_disjoint; eauto. esplits; eauto. }
-      { exfalso. eapply ModSem.step_return_disjoint; eauto. esplits; eauto. }
-      exploit ModSem.final_frame_dtm.
-      { eapply FINALTGT. }
-      { eapply FINAL. }
-      i; des. clarify. clear_tac.
-      inv STACK. ss.
-      exploit K; try apply RSREL; eauto.
+      econs; eauto; cycle 1.
+      { eapply lift_receptive_at.
+        admit "Add to ModSem.v". }
+      i. ss. des_ifs.
+      inv STEPSRC; ModSem.tac. ss.
+      inv STACK; ss. des_ifs.
+      determ_tac ModSem.final_frame_dtm. clear_tac.
+      exploit K; try apply SIMRETV; eauto.
       { etransitivity; eauto. }
-      { specialize (SAFESRC _ (star_refl _ _ _)).
-        des; ss.
-        { inv SAFESRC. }
-        inv SAFESRC; ModSem.tac. ss.
-        determ_tac ModSem.final_frame_dtm. erewrite <- mcompat_src in *; eauto.
-      }
-      i; des. exploit KSTEP; eauto. i; des.
+      i; des.
       esplits; eauto.
       + left. apply plus_one.
+        econs; eauto.
+        { admit "Add to semprops. / Modsem". }
         econs 4; ss; eauto.
-        erewrite <- mcompat_src in *; eauto.
       + right. eapply CIH; eauto.
         instantiate (1:= (SimMem.unlift sm_arg sm0)).
         econs; ss; cycle 1.
@@ -911,13 +754,11 @@ Section ADQSTEP.
         { etransitivity; eauto.
           eapply SimMem.unlift_spec; eauto.
           etransitivity; eauto. }
-        { erewrite mcompat_tgt in AFTER; eauto. determ_tac ModSem.after_external_dtm. eauto. }
+        { eauto. }
         { des_ifs.
           eapply mle_preserves_sim_ge; eauto.
           eapply SimMem.unlift_spec; eauto.
           etransitivity; eauto. }
-  Unshelve.
-    all: ss.
   Qed.
 
 End ADQSTEP.
@@ -934,8 +775,8 @@ Section ADQ.
   Hypothesis SIMPROG: ProgPair.sim pp.
   Let p_src := pp.(ProgPair.src).
   Let p_tgt := pp.(ProgPair.tgt).
-  Let sem_src := Sem.semantics p_src.
-  Let sem_tgt := Sem.semantics p_tgt.
+  Let sem_src := Sem.sem p_src.
+  Let sem_tgt := Sem.sem p_tgt.
 
   Theorem adequacy_local
     :
