proof/SimMemId.v
@@ -13,7 +13,7 @@ Require Import Asmregs.
 Require Import Integers.
 
 Require Import IntegersC LinkingC.
-Require Import SimDef SimSymb Skeleton Mod ModSem.
+Require Import SimSymb Skeleton Mod ModSem.
 Require SimSymbId.
 Require Import SimMem.
 
